src/coq/TopLevel.v
@@ -19,6 +19,7 @@ From ExtLib Require Import
      Data.Map.FMapAList.
 
 From Vellvm Require Import
+     TransformTypes
      DynamicTypes
      LLVMEvents
      Denotation
@@ -44,36 +45,36 @@ Export IO.DV.
 
 Open Scope string_scope.
 
-Definition allocate_globals (CFG: CFG.mcfg) (gs:list global) : LLVM _CFG D.genv :=
+Definition allocate_globals (gs:list (global dtyp)) : LLVM _CFG D.genv :=
   monad_fold_right
-    (fun (m:D.genv) (g:global) =>
-       vis (Alloca (D.eval_typ CFG (g_typ g))) (fun v => ret (D.ENV.add (g_ident g) v m))) gs (@D.ENV.empty _).
+    (fun (m:D.genv) (g:(global dtyp)) =>
+       vis (Alloca (g_typ _ g)) (fun v => ret (D.ENV.add (g_ident _ g) v m))) gs (@D.ENV.empty _).
 
 
 (* Who is in charge of allocating the addresses for external functions declared in this mcfg? *)
-Definition register_declaration (g:D.genv) (d:declaration) : LLVM _CFG D.genv :=
+Definition register_declaration (g:D.genv) (d:declaration dtyp) : LLVM _CFG D.genv :=
   (* SAZ TODO:  Don't allocate pointers for LLVM intrinsics declarations *)
-    vis (Alloca DTYPE_Pointer) (fun v => ret (D.ENV.add (dc_name d) v g)).
+    vis (Alloca DTYPE_Pointer) (fun v => ret (D.ENV.add (dc_name _ d) v g)).
 
 
-Definition initialize_globals (CFG: CFG.mcfg) (gs:list global) (g:D.genv) : LLVM _CFG unit :=
+Definition initialize_globals (gs:list (global dtyp)) (g:D.genv) : LLVM _CFG unit :=
   monad_fold_right
-    (fun (_:unit) (glb:global) =>
-       let dt := D.eval_typ CFG (g_typ glb) in
-       a <- lift_err ret (D.lookup_env g (g_ident glb)) ;;
+    (fun (_:unit) (glb:global dtyp) =>
+       let dt := (g_typ _ glb) in
+       a <- lift_err ret (D.lookup_env g (g_ident _ glb)) ;;
        dv <-
-           match (g_exp glb) with
+           match (g_exp _ glb) with
            | None => ret DVALUE_Undef
-           | Some e => D.denote_exp CFG g (Some dt) e
+           | Some e => D.denote_exp g (Some dt) e
            end ;;
        vis (Store a dv) ret)
     gs tt.
   
-Definition build_global_environment (CFG : CFG.mcfg) : LLVM _CFG D.genv :=
-  g <- allocate_globals CFG (m_globals CFG) ;;
+Definition build_global_environment (CFG : CFG.mcfg dtyp) : LLVM _CFG D.genv :=
+  g <- allocate_globals (m_globals _ _ CFG) ;;
   g1 <- monad_fold_right register_declaration
-       ((m_declarations CFG) ++ (List.map df_prototype (m_definitions CFG))) g;;
-  initialize_globals CFG (m_globals CFG) g1 ;;
+       ((m_declarations _ _ CFG) ++ (List.map (df_prototype _ _) (m_definitions _ _ CFG))) g;;
+  initialize_globals (m_globals _ _ CFG) g1 ;;
   ret g1.
 
 (* Local environment implementation *)
@@ -85,9 +86,9 @@ Definition function_env := FMapAList.alist dvalue D.function_denotation.
 (* -  let fid := (dc_name d) in *)
 (* -  liftM (fun fv => (fv, (df_args df, D.denote_cfg CFG g (df_instrs df)))) (D.lookup_env g fid). *)
 
-Definition address_one_function CFG (g:D.genv) (df : definition CFG.cfg) : err (dvalue * D.function_denotation) :=
-  let fid := (dc_name (df_prototype df)) in
-   liftM (fun fv => (fv, D.denote_function CFG g df)) (D.lookup_env g fid).
+Definition address_one_function (g:D.genv) (df : definition dtyp (CFG.cfg dtyp)) : err (dvalue * D.function_denotation) :=
+  let fid := (dc_name _ (df_prototype _ _ df)) in
+   liftM (fun fv => (fv, D.denote_function g df)) (D.lookup_env g fid).
    
 
 (* (for now) assume that [main (i64 argc, i8** argv)] 
@@ -98,13 +99,20 @@ Definition main_args := [DV.DVALUE_I64 (DynamicValues.Int64.zero);
                          DV.DVALUE_Addr (Memory.A.null)
                         ].
 
-Definition run_with_memory (prog: list (toplevel_entity (list block))) :
+Definition eval_typ (CFG:CFG.mcfg typ) (t:typ) : dtyp :=
+      TypeUtil.normalize_type_dtyp (m_type_defs _ _ CFG) t.
+
+Definition normalize_types (CFG:(CFG.mcfg typ)) : (CFG.mcfg dtyp) :=
+  TransformTypes.fmap_mcfg _ _ (eval_typ CFG) CFG.
+
+Definition run_with_memory (prog: list (toplevel_entity typ (list (block typ)))) :
   option (LLVM _MCFG2 (M.memory * (@L.stack local_env * DV.dvalue))) :=
-  let scfg := Vellvm.AstLib.modul_of_toplevel_entities prog in
-  mcfg <- CFG.mcfg_of_modul scfg ;;       
+    let scfg := Vellvm.AstLib.modul_of_toplevel_entities _ prog in
+    ucfg <- CFG.mcfg_of_modul _ scfg ;;
+    let mcfg := normalize_types ucfg in 
        let core_trace : LLVM _CFG dvalue :=
            'glbls <- build_global_environment mcfg ;;
-           'defns <- lift_err ret (map_monad (address_one_function mcfg glbls) (m_definitions mcfg)) ;;
+           'defns <- lift_err ret (map_monad (address_one_function glbls) (m_definitions _ _ mcfg)) ;;
            'addr <- lift_err ret (D.lookup_env glbls (Name "main")) ;;
            D.denote_mcfg defns DTYPE_Void addr main_args in
        let after_intrinsics_trace : LLVM _CFG dvalue := INT.interpret_intrinsics core_trace in
