src/coq/Transform.v
@@ -26,30 +26,36 @@ Definition mangle_ident (id:ident) : ident :=
   | ID_Local i => ID_Local (mangle_raw_id i)
   end.
 
-Definition mangle_instr (i:instr_id * instr) : (instr_id * instr) :=
+Section WithT.
+  Variable (T : Set).
+  
+
+Definition mangle_instr (i:instr_id * instr T) : (instr_id * instr T) :=
   match i with
   | _ => i
   end.
 
-Definition mangle_block (blk:block) : block :=
+Definition mangle_block (blk:block T) : block T :=
   blk.
 
-Definition mangle_blocks (blks:list block) : list block :=
+Definition mangle_blocks (blks:list (block T)) : list (block T) :=
   List.map mangle_block blks.
 
-Definition mangle_definition (d:definition (list block)) : definition (list block) :=
-  mk_definition _
-  (df_prototype d)
-  (df_args d)
-  (mangle_blocks (df_instrs d))
+Definition mangle_definition (d:definition T (list (block T))) : definition T (list (block T)) :=
+  mk_definition _ _
+  (df_prototype _ _ d)
+  (df_args _ _ d)
+  (mangle_blocks (df_instrs _ _ d))
 .
 
 
-Definition mangle_toplevel_entity (tle : toplevel_entity (list block)) : toplevel_entity (list block) :=
+Definition mangle_toplevel_entity (tle : toplevel_entity T (list (block T))) : toplevel_entity T (list (block T)) :=
   match tle with
-  | TLE_Definition d => TLE_Definition (mangle_definition d)
+  | TLE_Definition d => TLE_Definition _ _ (mangle_definition d)
   | _ => tle
   end.
 
-Definition transform (prog: list (toplevel_entity (list block))) : list (toplevel_entity (list block)) :=
+Definition transform (prog: list (toplevel_entity T (list (block T)))) : list (toplevel_entity T (list (block T))) :=
   List.map mangle_toplevel_entity prog.
+
+End WithT.
